Working example

Sample.fst
@@ -1,19 +1,168 @@
 module Sample
 
 open TLS.Curve25519
+open FStar.HyperStack.ST
+open FStar.Bytes
+open FStar.All
 
-let dhtest () =
-    let (gx, x) = keygen 4 in
-    let (gy, y) = keygen 4 in
-    let gxy = scalarmult y gx in
-    let gyx = scalarmult x gy in
-    //assert (gxy == gyx);
-    0
 
-// let pubshare k =
-//   let KSEC  ks = ks in S_EC ecg (ECGroup.pubshare #ecg ks)
-//   match k with
-//   | KSCC p  -> S_CC p
-//   | KS_X25519 k -> S_X25519 (TLS.Curve25519.pubshare k)
-//   | KSX448 p  -> S_X448 p
+//#set-options "--max_fuel 1000 --max_ifuel 1000 --z3rlimit 5000"
+// let dhtest () =
+//     let (gx, x) = keygen 4 in
+//     let (gy, y) = keygen 4 in
+//     let gxy = scalarmult y gx in
+//     let gyx = scalarmult x gy in
+//     assert (gxy == gyx);
+//     0
+
+// val multEq: s1:nat{FStar.Bytes.repr_bytes s1 <= 32} -> s2:nat{FStar.Bytes.repr_bytes s2 <= 32} -> 
+//     Lemma (requires(_->True))
+//         (ensures(scalarmult s2 (scalarmult s1 ))) 
+
+assume val deformat_point: bytes -> point
+assume val format_point: (p:point) -> (b:bytes{(deformat_point b) = p})
+
+// val multEq: p1:point -> s1:scalar -> s2:scalar ->
+//     Lemma (requires(True))
+//         (ensures((mul s2 (mul s1 p1)) = (mul s1 (mul s2 p1))))
+
+// val multEq: (s1: nat) (p1: point) (sc1: scalar) (s2: nat) (p2: point) (sc2: scalar) ->
+//     Lemma (requires(true)) 
+// ensures((p1, sc1) = keygen s1 /\ (p2, sc2) = keygen s2 ==> scalarmult sc1 p2 = scalarmult sc2 p1)
+
+// assume MultEq: forall (s1: nat) (p1: point) (sc1: scalar) (s2: nat) (p2: point) (sc2: scalar). {(p1, sc1) = keygen s1 /\ (p2, sc2) = keygen s2 ==> scalarmult sc1 p2 = scalarmult sc2 p1  }
+
+val clientHello: (s:nat{FStar.Bytes.repr_bytes s <= 32}) -> ST (bytes * scalar)
+    (requires (fun h0 -> True))
+    (ensures (fun h0 t h1 -> modifies_none h0 h1 /\ generated (snd t) (deformat_point (fst t)) s))
+let clientHello s =
+    let (gx, x) = keygen s in
+    ((format_point gx), x)
+
+val serverResponse: (s:nat{FStar.Bytes.repr_bytes s <= 32}) -> b:bytes -> ST (bytes * scalar * point)
+    (requires (fun h0 -> True))
+    (ensures (fun h0 tr h1 -> modifies_none h0 h1 /\ (
+        let (d, y, _) = tr in 
+        generated y (deformat_point d) s
+    ) /\ (
+        let (_, y, p) = tr in
+        composed y (deformat_point b) p
+    )))
+let serverResponse s b =
+    let (gy, y) = keygen s in
+    let gx = deformat_point b in
+    let gxy = mul y gx in
+    ((format_point gy), y, gxy)
+
+val clientConfirm: b:bytes -> x:scalar -> ST bytes
+    (requires (fun h0 -> True))
+    (ensures (fun h0 tb h1 -> modifies_none h0 h1 /\ composed x (deformat_point b) (deformat_point tb) ))
+let clientConfirm b x =
+    let gy = deformat_point b in
+    let gyx = mul x gy in
+    (format_point gyx)
+
+val serverConfirm: b:bytes -> gxy:point -> Tot bool
+let serverConfirm b gxy =
+    let gyx = deformat_point b in
+    (gyx = gxy)
+
+let ecdhtest =
+    let sec1 = 1 in
+    let sec2 = 2 in
+    let (bgx, x) = (clientHello sec1) in
+    let (bgy, y, gxy) = (serverResponse sec2 bgx) in
+    let bgyx = (clientConfirm bgy x) in
+    mulEq x y (deformat_point bgx) (deformat_point bgy) gxy (deformat_point bgyx) sec1 sec2;
+    let eq = (serverConfirm bgyx gxy) in
+    assert (eq)
+    
+
+
+// val sendClientHello: s:nat{FStar.Bytes.repr_bytes s <= 32} -> ST keyshare
+//     (requires (fun h0 -> True))
+//     (ensures (fun h0 _ h1 -> modifies_none h0 h1))
+
+// let sendClientHello s =
+//     keygen s
+
+// val recieveClientHello: (s:nat{FStar.Bytes.repr_bytes s <= 32}) -> gx:point -> ST (point * point)
+//     (requires (fun h0 -> True))
+//     (ensures (fun h0 _ h1 -> modifies_none h0 h1))
+
+// let recieveClientHello s gx =
+//     let (gy, y) = keygen s in
+//     let gxy = mul y gx in
+//     (gy, gxy)
+
+// val sendServerResponse: gy:point -> point
+// let sendServerResponse gy =
+//     gy
+
+// val recieveServerResponse: gy: point -> x:scalar -> ST point
+//     (requires (fun h0 -> True))
+//     (ensures (fun h0 _ h1 -> modifies_none h0 h1))
+// let recieveServerResponse gy x =
+//     mul x gy
+
+// // val sendClientConfirm: gxy:nat -> Tot hash
+// // let sendClientConfirm gxy =
+// //     let h = hashNat gxy in
+// //     h
+
+// // val recieveClientConfirm: gxy_hash:hash -> gxy: nat -> Tot bool
+// // let recieveClientConfirm gxy_hash gxy =
+// //     let gxy_hash' = hashNat gxy in
+// //     gxy_hash = gxy_hash'
+
+// #set-options "--max_fuel 1000 --max_ifuel 1000 --z3rlimit 5000"
+// let dhtest =
+
+//     //Client hello    
+//     let (gx, x) = sendClientHello 8 in
+//     //assert (verify client_keypair.pkey gx gx_sign) in
+
+//     //Server response
+//     let (gy, server_gxy) = recieveClientHello 9 gx in
+//     let gy' = sendServerResponse gy in
+
+//     //Client confirm
+//     let client_gxy = recieveServerResponse gy' x in
+//     // let client_gxy_hash = sendClientConfirm client_gxy in
+
+//     let b = format_point gx in
+//     assert (gx = deformat_point b)
+
+
+    // //Server confirm
+    // let gxyHashesEqual = recieveClientConfirm client_gxy_hash server_gxy in
+    // assert gxyHashesEqual
+    //assert(client_gxy = server_gxy)
+
+// #set-options "--max_fuel 1000 --max_ifuel 1000 --z3rlimit 5000"
+// let dhtest () =
+//     let sec1 = 1 in
+//     let sec2 = 2 in
+//     let (gx, x) = (keygen sec1) in
+//     let (gy, y) = (keygen sec2) in
+//     (mulEq3 sec1 sec2);
+//     assert((mul y gx) <> (mul x gy))
+    //assert (false)
+    // let (gx, x) = keygen 4 in
+    // let (gy, y) = keygen 5 in
+    // // let gxy = mul y gx in
+    // // let gyx = mul x gy in
+    // // assert (generated x gx 4);
+    // assert ((mul y gx) = (mul x gy));
+    
+
+//# use corecrypto to get ecDH
+//# send recieve bytes (repr takes nat -> bytes and vice versa)
+//# find props/guarantees: 
+//# -- ***secrecy ?? keys not revealed to attacker
+// -- perfect forward secr
+// -- post-compromised secresy (device compr for a while)
+//    -- recover after compromise (key-rotation)
+// -- key-compromising impersonofication: for the client sessions attacker cannot get sessionkey (x gx gxy)
+// -- session key independence: if the attacker knows a sessionkey, he does not learn anything about keys of any other sesions
 
