TLS.Curve25519.fst
@@ -1,6 +1,6 @@
 module TLS.Curve25519
 
-open EverCrypt
+//open EverCrypt
 
 open FStar.Int32
 open FStar.Bytes
@@ -15,33 +15,63 @@ type scalar = lbytes 32
 type point = lbytes 32
 type keyshare = point * scalar
 
+// type eqPoint = hasEq point
+// type eqBytes = hasEq (lbytes 32)
+
 let pubshare (k:keyshare) : Tot point = fst k
 
-let scalarmult (secret:Bytes.lbytes 32) (point:Bytes.lbytes 32)
-  : ST (lbytes 32)
-  (requires (fun h -> True))
-  (ensures (fun h0 _ h1 -> modifies_none h0 h1)) =
-  push_frame ();
-  let lp = B.len point in
-  let ls = B.len secret in
-  let pb = LB.alloca 0uy lp in
-  let sb = LB.alloca 0uy ls in
-  let out = LB.alloca 0uy 32ul in
-  B.store_bytes point pb;
-  B.store_bytes secret sb;
-  assume false;
-  ignore (EverCrypt.Curve25519.ecdh out sb pb);
-  pop_frame (); B.of_buffer 32ul out
+assume val generated (sc:scalar) (p:point) (i:nat{FStar.Bytes.repr_bytes i <= 32}): bool
+assume val keygen (i:nat{FStar.Bytes.repr_bytes i <= 32}) : (ks:keyshare{ generated (snd ks) (fst ks) i  })
+assume val composed (k:scalar) (p:point) (tp:point) : bool
+assume val mul (k:scalar) (p:point) : (tp:point{composed k p tp})
 
-let keygen (i:nat{FStar.Bytes.repr_bytes i <= 32}) : ST keyshare
-  (requires (fun h0 -> True))
-  (ensures (fun h0 _ h1 -> modifies_none h0 h1))
-  =
-  let s : lbytes 32 = bytes_of_int 32 i in //sample32 32ul in
-  let basepoint = Bytes.create 1ul 9uy @| Bytes.create 31ul 0uy in
-  scalarmult s basepoint, s
+// let (gx, x) = keygen 4 in
+//     let (gy, y) = keygen 5 in
+//     let gxy = mul y gx in
+//     let gyx = mul x gy in
+//     // assert (generated x gx 4);
+//     assert (gxy = gyx);
 
-let mul (k:scalar) (p:point) : ST point
-  (requires (fun h0 -> True))
-  (ensures (fun h0 _ h1 -> modifies_none h0 h1))
-  = scalarmult k p
+// val mulEq2: k1:scalar -> k2:scalar -> p1:point -> p2:point ->
+//   Lemma (requires(k1=k2 /\ p1=p2))
+//       (ensures(mul k1 p1 = mul k2 p2))
+    
+val mulEq3: sec1:nat -> sec2:nat ->
+    Lemma (requires(True))
+        (ensures(
+          let (gx, x) = keygen sec1 in
+          let (gy, y) = keygen sec2 in
+          ((mul y gx) = (mul x gy))))
+
+val mulEq: x:scalar -> y:scalar -> gx:point -> gy:point -> gxy:point -> gyx:point -> (s1:nat{FStar.Bytes.repr_bytes s1 <= 32}) -> ( s2:nat{FStar.Bytes.repr_bytes s2 <= 32}) ->
+  Lemma (requires(generated x gx s1 /\ generated y gy s2 /\ composed y gx gxy /\ composed x gy gyx))
+      (ensures(gxy = gyx))
+
+// let scalarmult (secret:Bytes.lbytes 32) (point:Bytes.lbytes 32)
+//   : ST (lbytes 32)
+//   (requires (fun h -> True))
+//   (ensures (fun h0 _ h1 -> modifies_none h0 h1)) =
+//   push_frame ();
+//   let lp = B.len point in
+//   let ls = B.len secret in
+//   let pb = LB.alloca 0uy lp in
+//   let sb = LB.alloca 0uy ls in
+//   let out = LB.alloca 0uy 32ul in
+//   B.store_bytes point pb;
+//   B.store_bytes secret sb;
+//   assume false;
+//   ignore (EverCrypt.Curve25519.ecdh out sb pb);
+//   pop_frame (); B.of_buffer 32ul out
+
+// let keygen (i:nat{FStar.Bytes.repr_bytes i <= 32}) : ST keyshare
+//   (requires (fun h0 -> True))
+//   (ensures (fun h0 _ h1 -> modifies_none h0 h1))
+//   =
+//   let s : lbytes 32 = bytes_of_int 32 i in //sample32 32ul in
+//   let basepoint = Bytes.create 1ul 9uy @| Bytes.create 31ul 0uy in
+//   scalarmult s basepoint, s
+
+// let mul (k:scalar) (p:point) : ST point
+//   (requires (fun h0 -> True))
+//   (ensures (fun h0 _ h1 -> modifies_none h0 h1))
+//   = scalarmult k p
